

Exercise 4.1

$$\rightarrow \text{let } d' \leftarrow \frac{d}{\gcd(d, p-1)} \quad p'-1 \leftarrow \frac{p-1}{\gcd(d, p-1)} \quad (i)$$

$$\Rightarrow x^{d'} = a \text{ in } \mathbb{Z}_{p'} \text{ has a unique root } = a^{k'} \\ \text{where } d'k' \equiv 1 \pmod{p'-1}$$

$$\text{if } a^{k'} \neq 1 \Rightarrow \text{No sol}^n$$

$$\text{else } k', 2k', 3k' \dots \gcd(d, p-1)k' \text{ are all} \\ \text{powers of } (p) \text{ s.t. } a^p \text{ is a root. (ii)}$$

$$\therefore 0 \text{ sol}^n \text{ or } \gcd(d, p-1) \text{ sol}^n$$

Exercise 4.2

\rightarrow Every 2 steps, degree reduces by 1
cost of division = $d \log d$

$$\Rightarrow O(2 \cdot d + d^2 \cdot \log^2(p))$$

each step d terms

requiring $d \cdot \log p$ time
computation

$$n = b_r$$

$$s = \log b = 1.9 \text{ (ii)}$$

$$\log \Sigma m \quad \varepsilon = r$$

$$\text{calculate } d_1$$

$$1 = \log m$$

$$e$$

Exercise 4.3

(i) \mathbb{Z}_{67}

(i) $x^5 = 3, \quad (x^d = a)$

$d=5 \quad p-1=66 \Rightarrow \gcd(d, p-1)=1$

$\therefore 5k = 1 \pmod{66}$

$\Rightarrow 5k - 66y = 1$

$(-13, -1)$

$\therefore -13 \equiv 54 \pmod{67}$

$\therefore x = 3^{54} \text{ is a solution}$

(ii) $x^3 = 2$

$x^d = a$

$d=3 \quad p-1=66 \quad \gcd(d, p-1)=3$

$d'=1 \quad p'-1=22$

$\therefore x = 2 \text{ in } \mathbb{Z}_{23}$

solution is 2^{22}

 \Rightarrow other solutions

$2^{22} \text{ in } \mathbb{Z}_{23} = 37 \neq 1$

$2^0=1, 2^1=2, 2^2=4, 2^4=16, 2^8=10, 2^{16}=8$

$2^{20}=18=(-5)$

$2^{22}=(-20)=3$

No solution

(iii) $x^2 = 3$

$x^d = a$

$d=2 \quad p-1=66 \Rightarrow \gcd=2$

$x = 3 \text{ in } \mathbb{Z}_{34}$

$3^{33} \text{ in } \mathbb{Z}_{67} = -1 \therefore \text{No solution}$

(iv) $x^2 = 17$

$\rightarrow 17^{33} \pmod{67} = 1$

has 2 solutions

$x = 33$ and 34

~~17 is a solution~~

~~17 is a solution~~

~~$(5-x)(x) - (1-x)(x) = (5-x) - (1-x)$~~

~~$(5-x)(x) - (1-x)(x) = (5-x) - (1-x)$~~

Exercise 4.4

\rightarrow

$h(x) - f(x) = \alpha(x) q(x)$

$h(x) - g(x) = \beta(x) r(x)$

$\therefore h(x) = f(x) + \alpha(x) q(x) = g(x) + \beta(x) r(x)$

\Rightarrow We can solve $\alpha(x) q(x) - \beta(x) r(x) = g(x) - f(x)$

using Euclid's Algorithm to find $\alpha(x), \beta(x)$

This is possible because $q(x), r(x)$ are irreducible, \therefore no common factors,

hence $\gcd = 1$. By Bezout's lemma $\alpha(x), \beta(x)$ exist

Exercise 4.5

(a) $x^2 + 1$ in \mathbb{Z}_{11} , check if $x^2 = 10$ has solutions

$10^{\frac{10}{2}} = 10^5 \pmod{11}$

$10^1 = 10, 10^2 = 1, 10^4 = 1 \Rightarrow 10^5 = 10 \neq 1$

\therefore No soln hence irreducible

ally $x^2 = 2$

\Rightarrow check $25 = 32 \pmod{11} = -1$

hence no soln

(b) $f(x) - (x+2) = \alpha(x)(x^2+1)$

$f(x) - (2x-3) = \beta(x)(x^2-2)$

$\Rightarrow \cancel{f(x)} - (2x-3) - (x+2) = \alpha(x)(x^2+1) - \beta(x)(x^2-2)$

$\Rightarrow x-5 = \alpha(x)(x^2+1) - \beta(x)(x^2-2)$

first solve for α, β

a	b	q	x^2	y	v
x^2+1	x^2-2	1	1	0	1
x^2-2	3	$4x^2+7$	0	1	-1
3	0	-	1	-1	

$$\begin{array}{r} 1 \\ x^2-2 \overline{) x^2+1} \\ \underline{x^2-2} \\ 3 \end{array} \quad \begin{array}{r} 4x^2+7 \\ x^2-2 \overline{) 4x^2+7} \\ \underline{x^2-2} \\ 10 \\ \underline{10} \\ 0 \end{array}$$

$\therefore \alpha(x)=1 \quad \beta(x)=1 \Rightarrow 1(x^2+1) - 1(x^2-2) = 3$

$\therefore 3^{-1} = 4$

$\therefore 4(x^2+1) - 4(x^2-2) = 1$

to solve $(x-5)$ just multiply

$4(x-5)(x^2+1) - 4(x-5)(x^2-2) = x-5$

$\therefore f(x) = x+2 + 4(x-5)(x^2+1)$

$= x+2 + 4(x^3-5x^2+x-5)$

$= 4x^3 - 20x^2 + 5x - 18$

$= 4x^3 + 2x^2 + 5x + 4$